Make dlist parametric in a predicate on data

lib_list/ArrayList.fst
@@ -34,8 +34,10 @@ let null_ptr : US.t = 0sz
 /// The [visited] argument is needed to ensure termination, it corresponds to the set of cells
 /// previously visited. Acyclicity is specified by guaranteeing that we do not visit a cell twice.
 /// [prev] corresponds to the index of the previous cell.
+/// The list is parametric in a predicate [pred], operating on the data, that all elements
+/// of the list must satisfy
 /// Note, as a convention, we consider that NULL corresponds to 0, and do not store anything there
-let rec is_dlist' (#a:Type0) (hd:nat) (s:Seq.seq (cell a)) (prev:nat)
+let rec is_dlist' (#a:Type0) (pred: a -> prop) (hd:nat) (s:Seq.seq (cell a)) (prev:nat)
   (visited:FS.set nat{Seq.length s >= FS.cardinality visited})
   : Tot prop (decreases (Seq.length s - FS.cardinality visited)) =
   // Null case.
@@ -50,13 +52,18 @@ let rec is_dlist' (#a:Type0) (hd:nat) (s:Seq.seq (cell a)) (prev:nat)
     else
       let cur = Seq.index s hd in
       let next = US.v cur.next in
-      is_dlist' next s hd (FS.insert hd visited) /\ US.v cur.prev == prev
+      // The tail of the list is a doubly linked list
+      is_dlist' pred next s hd (FS.insert hd visited) /\
+      // The previous field correctly points to the previous element
+      US.v cur.prev == prev /\
+      // The data of the list satisfies the predicate [pred]
+      pred cur.data
 
 /// The toplevel specification of being a list
 /// When [hd] is the head pointer of the list, the set of visited nodes
 /// is initially empty, and the prev "pointer" should be "NULL"
-let is_dlist (#a:Type0) (hd:nat) (s:Seq.seq (cell a)) : prop =
-  is_dlist' hd s null FS.emptyset
+let is_dlist (#a:Type0) (pred: a -> prop)  (hd:nat) (s:Seq.seq (cell a)) : prop =
+  is_dlist' pred hd s null FS.emptyset
 
 let rec mem' (#a:Type0) (x:nat) (hd:nat) (s:Seq.seq (cell a))
   (visited:FS.set nat{Seq.length s >= FS.cardinality visited})
@@ -83,21 +90,24 @@ let write_data (#a:Type0) (c:cell a) (v:a) : cell a =
   {c with data = v}
 
 let next_ptr (#a:Type)
+  (pred:a -> prop)
   (hd:nat)
   (s:Seq.seq (cell a))
   (prev:nat)
   (visited:FS.set nat{Seq.length s >= FS.cardinality visited})
 
   : Ghost nat
-          (requires is_dlist' hd s prev visited /\ hd <> null)
+          (requires is_dlist' pred hd s prev visited /\ hd <> null)
           (ensures fun _ -> True)
   = US.v (Seq.index s hd).next
 
 (** Lemmas about the dlist predicate *)
 
 /// Framing lemma: Only changing the `data` field of a cell
-/// does not change the structure of the doubly linked list
+/// does not change the structure of the doubly linked list,
+/// as long as we store an element satisfying [pred]
 let rec lemma_write_data_frame' (#a:Type0)
+  (pred: a -> prop)
   (hd:nat)
   (s:Seq.seq (cell a))
   (prev:nat)
@@ -105,8 +115,8 @@ let rec lemma_write_data_frame' (#a:Type0)
   (v:a)
   (visited:FS.set nat{Seq.length s >= FS.cardinality visited})
   : Lemma
-      (requires is_dlist' hd s prev visited)
-      (ensures is_dlist' hd (Seq.upd s idx (write_data (Seq.index s idx) v)) prev visited)
+      (requires is_dlist' pred hd s prev visited /\ pred v)
+      (ensures is_dlist' pred hd (Seq.upd s idx (write_data (Seq.index s idx) v)) prev visited)
       (decreases (Seq.length s - FS.cardinality visited))
   = let s' = Seq.upd s idx (write_data (Seq.index s idx) v) in
     if hd = null then ()
@@ -116,23 +126,25 @@ let rec lemma_write_data_frame' (#a:Type0)
         let next1 = US.v (Seq.index s hd).next in
         let next2 = US.v (Seq.index s' hd).next in
         assert (next1 == next2);
-        lemma_write_data_frame' next1 s hd idx v (FS.insert hd visited)
+        lemma_write_data_frame' pred next1 s hd idx v (FS.insert hd visited)
 
 val lemma_write_data_frame (#a:Type0)
+  (pred: a -> prop)
   (hd:nat)
   (s:Seq.seq (cell a))
   (idx:nat{idx < Seq.length s})
   (v:a)
   : Lemma
-      (requires is_dlist hd s)
-      (ensures is_dlist hd (Seq.upd s idx (write_data (Seq.index s idx) v)))
+      (requires is_dlist pred hd s /\ pred v)
+      (ensures is_dlist pred hd (Seq.upd s idx (write_data (Seq.index s idx) v)))
 
-let lemma_write_data_frame #a hd s idx v =
-  lemma_write_data_frame' hd s null idx v FS.emptyset
+let lemma_write_data_frame #a pred hd s idx v =
+  lemma_write_data_frame' pred hd s null idx v FS.emptyset
 
 let null_or_valid (#a:Type) (ptr:nat) (s:Seq.seq (cell a)) = ptr = null \/ ptr < Seq.length s
 
 val lemma_mem_valid_or_null_next_prev' (#a:Type0)
+  (pred: a -> prop)
   (hd:nat)
   (s:Seq.seq (cell a))
   (prev: nat)
@@ -140,7 +152,7 @@ val lemma_mem_valid_or_null_next_prev' (#a:Type0)
   (idx:nat)
   : Lemma
       (requires
-        is_dlist' hd s prev visited /\
+        is_dlist' pred hd s prev visited /\
         mem' idx hd s visited /\
         null_or_valid prev s /\
         not (FS.mem idx visited))
@@ -148,12 +160,11 @@ val lemma_mem_valid_or_null_next_prev' (#a:Type0)
         (let cell = Seq.index s idx in
         null_or_valid (US.v cell.next) s /\
         null_or_valid (US.v cell.prev) s /\
-//        True)
         (US.v cell.next == null \/ mem' (US.v cell.next) hd s visited))
       )
       (decreases (Seq.length s - FS.cardinality visited))
 
-let rec lemma_mem_valid_or_null_next_prev' #a hd s prev visited idx
+let rec lemma_mem_valid_or_null_next_prev' #a pred hd s prev visited idx
   =
   assert (not (idx = null || idx >= Seq.length s));
   let cur = Seq.index s hd in
@@ -166,28 +177,30 @@ let rec lemma_mem_valid_or_null_next_prev' #a hd s prev visited idx
     assert (~ (mem' idx null s visited))
   end else begin
     assert (not (FS.cardinality visited = Seq.length s || FS.mem hd visited || hd >= Seq.length s));
-    assert (is_dlist' next s hd (FS.insert hd visited));
+    assert (is_dlist' pred next s hd (FS.insert hd visited));
     assert (mem' idx next s (FS.insert hd visited));
-    lemma_mem_valid_or_null_next_prev' #a next s hd (FS.insert hd visited) idx
+    lemma_mem_valid_or_null_next_prev' pred next s hd (FS.insert hd visited) idx
   end
 
 val lemma_mem_valid_or_null_next_prev (#a:Type0)
+  (pred: a -> prop)
   (hd:nat)
   (s:Seq.seq (cell a))
   (idx:nat)
   : Lemma
-      (requires is_dlist hd s /\ mem idx hd s)
+      (requires is_dlist pred hd s /\ mem idx hd s)
       (ensures
         (let cell = Seq.index s idx in
         null_or_valid (US.v cell.prev) s /\ null_or_valid (US.v cell.next) s)
       )
 
-let lemma_mem_valid_or_null_next_prev #a hd s idx =
-  lemma_mem_valid_or_null_next_prev' hd s null FS.emptyset idx
+let lemma_mem_valid_or_null_next_prev #a pred hd s idx =
+  lemma_mem_valid_or_null_next_prev' pred hd s null FS.emptyset idx
 
 /// If idx belongs to the dlist, then either it is the head of the dlist
 /// or its prev pointer does not belong to the visited set
 val lemma_dlist_head_or_prev_not_visited (#a:Type0)
+  (pred: a -> prop)
   (hd:nat)
   (s:Seq.seq (cell a))
   (prev: nat)
@@ -195,7 +208,7 @@ val lemma_dlist_head_or_prev_not_visited (#a:Type0)
   (idx:nat)
   : Lemma
       (requires
-        is_dlist' hd s prev visited /\
+        is_dlist' pred hd s prev visited /\
         mem' idx hd s visited /\
         null_or_valid prev s /\
         not (FS.mem idx visited))
@@ -206,23 +219,24 @@ val lemma_dlist_head_or_prev_not_visited (#a:Type0)
       )
       (decreases (Seq.length s - FS.cardinality visited))
 
-let rec lemma_dlist_head_or_prev_not_visited hd s prev visited idx =
+let rec lemma_dlist_head_or_prev_not_visited pred hd s prev visited idx =
   if idx = hd || hd = null then ()
   else
     let cur = Seq.index s hd in
     let next = US.v cur.next in
-    lemma_dlist_head_or_prev_not_visited next s hd (FS.insert hd visited) idx
+    lemma_dlist_head_or_prev_not_visited pred next s hd (FS.insert hd visited) idx
 
 (** Functional specifications of the more complicated functions *)
 
 /// A ghost specification of the insertion function for doubly linked lists
 let insert_spec (#a:Type)
+  (pred: a -> prop)
   (s:Seq.seq (cell a))
   (hd:US.t{hd == null_ptr \/ US.v hd < Seq.length s})
   (idx:US.t{idx <> null_ptr /\ US.v idx < Seq.length s})
   (v:a)
   : Ghost (Seq.seq (cell a))
-         (requires is_dlist (US.v hd) s /\ ~ (mem (US.v idx) (US.v hd) s))
+         (requires is_dlist pred (US.v hd) s /\ ~ (mem (US.v idx) (US.v hd) s))
          (ensures fun _ -> True)
   = let cell = {data = v; prev = null_ptr; next = hd} in
     let s = Seq.upd s (US.v idx) cell in
@@ -235,6 +249,7 @@ let insert_spec (#a:Type)
 
 /// A ghost specification of the remove function for doubly linked lists
 let remove_spec (#a:Type)
+  (pred: a -> prop)
   (hd:nat)
   (s:Seq.seq (cell a))
   (prev:nat)
@@ -242,14 +257,14 @@ let remove_spec (#a:Type)
   (visited:FS.set nat{Seq.length s >= FS.cardinality visited})
   : Ghost (Seq.seq (cell a))
          (requires
-           is_dlist' hd s prev visited /\
+           is_dlist' pred hd s prev visited /\
            mem' idx hd s visited /\
            null_or_valid prev s /\
            not (FS.mem idx visited))
          (ensures fun s' -> Seq.length s == Seq.length s')
          =
   let cell = Seq.index s idx in
-  lemma_mem_valid_or_null_next_prev' hd s prev visited idx;
+  lemma_mem_valid_or_null_next_prev' pred hd s prev visited idx;
   let s =
     if cell.next <> null_ptr then
       // Next is not null, we need to update it
@@ -271,6 +286,7 @@ let remove_spec (#a:Type)
 (** Functional correctness lemmas for insert and remove *)
 
 let rec lemma_dlist_upd' (#a:Type)
+  (pred: a -> prop)
   (s:Seq.seq (cell a))
   (hd:nat{hd == null \/ hd < Seq.length s})
   (idx:nat{idx <> null /\ idx < Seq.length s})
@@ -280,12 +296,12 @@ let rec lemma_dlist_upd' (#a:Type)
   (v: cell a)
   : Lemma
   (requires
-    is_dlist' hd s prev visited /\
+    is_dlist' pred hd s prev visited /\
     ~ (mem' idx hd s visited) /\
     ~ (mem' other hd s visited))
   (ensures (
     let s' = Seq.upd s idx v in
-    is_dlist' hd s' prev visited /\
+    is_dlist' pred hd s' prev visited /\
     ~ (mem' idx hd s' visited) /\
     ~ (mem' other hd s' visited))
     )
@@ -298,12 +314,13 @@ let rec lemma_dlist_upd' (#a:Type)
   else begin
     let cur = Seq.index s hd in
     let next = cur.next in
-    assert (is_dlist' (US.v next) s hd (FS.insert hd visited));
+    assert (is_dlist' pred (US.v next) s hd (FS.insert hd visited));
     assert (~ (mem' idx hd s (FS.insert hd visited)));
-    lemma_dlist_upd' s (US.v next) idx hd other (FS.insert hd visited) v
+    lemma_dlist_upd' pred s (US.v next) idx hd other (FS.insert hd visited) v
   end
 
 let lemma_dlist_upd (#a:Type)
+  (pred: a -> prop)
   (s:Seq.seq (cell a))
   (hd:nat{hd == null \/ hd < Seq.length s})
   (idx:nat{idx <> null /\ idx < Seq.length s})
@@ -311,17 +328,17 @@ let lemma_dlist_upd (#a:Type)
   (v: cell a)
   : Lemma
   (requires
-    is_dlist hd s /\
+    is_dlist pred hd s /\
     ~ (mem idx hd s) /\
     ~ (mem other hd s)
     )
   (ensures (
     let s' = Seq.upd s idx v in
-    is_dlist hd s' /\
+    is_dlist pred hd s' /\
     ~ (mem idx hd s') /\
     ~ (mem other hd s')
     ))
-  = lemma_dlist_upd' s hd idx null other FS.emptyset v
+  = lemma_dlist_upd' pred s hd idx null other FS.emptyset v
 
 /// If we have a finiteset of elements smaller than a given n,
 /// and one element is not in the set, then the cardinality is not n
@@ -345,6 +362,7 @@ let lemma_finiteset_full_n (n:nat) (i:nat{i < n}) (s:FS.set nat)
      cardinality (difference s s_full) + cardinality (difference s_full s) + cardinality (intersection s s_full)))
 
 let rec lemma_dlist_insert_visited (#a:Type)
+  (pred: a -> prop)
   (s:Seq.seq (cell a))
   (hd:nat{hd == null \/ hd < Seq.length s})
   (idx:nat{idx <> null /\ idx < Seq.length s})
@@ -353,10 +371,10 @@ let rec lemma_dlist_insert_visited (#a:Type)
   : Lemma
   (requires
     (forall i. FS.mem i visited ==> i < Seq.length s) /\
-    is_dlist' hd s prev visited /\
+    is_dlist' pred hd s prev visited /\
     ~ (mem' idx hd s visited))
   (ensures
-    is_dlist' hd s prev (FS.insert idx visited) /\
+    is_dlist' pred hd s prev (FS.insert idx visited) /\
     ~ (mem' idx hd s (FS.insert idx visited)))
   (decreases (Seq.length s - FS.cardinality visited))
   =
@@ -365,7 +383,7 @@ let rec lemma_dlist_insert_visited (#a:Type)
   else begin
     let cur = Seq.index s hd in
     let next = cur.next in
-    assert (is_dlist' (US.v next) s hd (FS.insert hd visited));
+    assert (is_dlist' pred (US.v next) s hd (FS.insert hd visited));
     assert (~ (mem' idx hd s (FS.insert hd visited)));
 
     if US.v next = null then (
@@ -373,7 +391,7 @@ let rec lemma_dlist_insert_visited (#a:Type)
     )
     else begin
       assert (FS.cardinality (FS.insert hd visited) < Seq.length s);
-      lemma_dlist_insert_visited s (US.v next) idx hd (FS.insert hd visited);
+      lemma_dlist_insert_visited pred s (US.v next) idx hd (FS.insert hd visited);
       // Need to explicitly introduce Set extensionality
       assert (
         FS.insert hd (FS.insert idx visited)
@@ -384,6 +402,7 @@ let rec lemma_dlist_insert_visited (#a:Type)
   end
 
 let rec lemma_dlist_remove_visited (#a:Type)
+  (pred: a -> prop)
   (s:Seq.seq (cell a))
   (hd:nat{hd == null \/ hd < Seq.length s})
   (idx:nat{idx <> null /\ idx < Seq.length s})
@@ -392,10 +411,10 @@ let rec lemma_dlist_remove_visited (#a:Type)
   : Lemma
   (requires
     (forall i. FS.mem i visited ==> i < Seq.length s) /\
-    is_dlist' hd s prev (FS.insert idx visited) /\
+    is_dlist' pred hd s prev (FS.insert idx visited) /\
     ~ (mem' idx hd s (FS.insert idx visited)))
   (ensures
-    is_dlist' hd s prev visited /\
+    is_dlist' pred hd s prev visited /\
     ~ (mem' idx hd s visited))
   (decreases (Seq.length s - FS.cardinality visited))
   = if hd = null then ()
@@ -411,13 +430,14 @@ let rec lemma_dlist_remove_visited (#a:Type)
             `FS.equal`
           FS.insert hd (FS.insert idx visited)
         );
-        lemma_dlist_remove_visited s (US.v next) idx hd (FS.insert hd visited)
+        lemma_dlist_remove_visited pred s (US.v next) idx hd (FS.insert hd visited)
       end
     end
 
 /// If an element belongs to the visited set, then it
 /// does not belong to the dlist
 let rec lemma_mem_not_in_visited (#a:Type)
+  (pred: a -> prop)
   (s:Seq.seq (cell a))
   (hd:nat)
   (prev:nat)
@@ -425,7 +445,7 @@ let rec lemma_mem_not_in_visited (#a:Type)
   (ptr:nat)
   : Lemma
   (requires
-    is_dlist' hd s prev visited /\
+    is_dlist' pred hd s prev visited /\
     FS.mem ptr visited
   )
   (ensures
@@ -435,16 +455,17 @@ let rec lemma_mem_not_in_visited (#a:Type)
     else
       let cur = Seq.index s hd in
       let next = cur.next in
-      lemma_mem_not_in_visited s (US.v next) hd (FS.insert hd visited) ptr
+      lemma_mem_not_in_visited pred s (US.v next) hd (FS.insert hd visited) ptr
 
 let lemma_dlist_mem_uniq (#a:Type)
+  (pred: a -> prop)
   (s:Seq.seq (cell a))
   (hd:nat{hd <> null \/ hd < Seq.length s})
   (prev: nat)
   (visited: FS.set nat{FS.cardinality visited < Seq.length s})
   : Lemma
   (requires
-    is_dlist' hd s prev visited
+    is_dlist' pred hd s prev visited
   )
   (ensures (
     let cur = Seq.index s hd in
@@ -457,68 +478,70 @@ let lemma_dlist_mem_uniq (#a:Type)
     let cur = Seq.index s hd in
     let next = cur.next in
     assert (not (FS.mem hd visited));
-    assert (is_dlist' (US.v next) s hd (FS.insert hd visited));
-    lemma_mem_not_in_visited s (US.v next) hd (FS.insert hd visited) hd
+    assert (is_dlist' pred (US.v next) s hd (FS.insert hd visited));
+    lemma_mem_not_in_visited pred s (US.v next) hd (FS.insert hd visited) hd
 
 /// If a dlist is well-formed, the prev element does not belong to
 /// the list
 let lemma_dlist_prev_not_mem (#a:Type)
+  (pred: a -> prop)
   (s:Seq.seq (cell a))
   (hd:nat)
   (prev:nat)
   (visited:FS.set nat{FS.cardinality visited <= Seq.length s})
   : Lemma
   (requires
-    is_dlist' hd s prev visited
+    is_dlist' pred hd s prev visited
   )
   (ensures
     ~ (mem' prev hd s visited))
   (decreases (Seq.length s - FS.cardinality visited))
   = if hd = null || prev = null then ()
-    else lemma_mem_not_in_visited s hd prev visited prev
+    else lemma_mem_not_in_visited pred s hd prev visited prev
 
 /// Functional correctness of the insert_spec function:
 /// The resulting list is still a doubly linked list.
 /// Note, proving that the element was added is trivial, so we do not include it here
 let lemma_insert_spec (#a:Type)
+  (pred: a -> prop)
   (s:Seq.seq (cell a))
   (hd:US.t{hd == null_ptr \/ US.v hd < Seq.length s})
   (idx:US.t{idx <> null_ptr /\ US.v idx < Seq.length s})
   (v:a)
-  : Lemma (requires is_dlist (US.v hd) s /\ ~ (mem (US.v idx) (US.v hd) s))
-          (ensures is_dlist (US.v idx) (insert_spec s hd idx v))
+  : Lemma (requires pred v /\ is_dlist pred (US.v hd) s /\ (~ (mem (US.v idx) (US.v hd) s)))
+          (ensures is_dlist pred (US.v idx) (insert_spec pred s hd idx v))
   =
-  assert (is_dlist' (US.v hd) s null FS.emptyset);
+  assert (is_dlist' pred (US.v hd) s null FS.emptyset);
   let cell = {data = v; prev = null_ptr; next = hd} in
   let s' = Seq.upd s (US.v idx) cell in
-  lemma_dlist_upd s (US.v hd) (US.v idx) (US.v idx) cell;
-  assert (is_dlist' (US.v hd) s' null FS.emptyset);
+  lemma_dlist_upd pred s (US.v hd) (US.v idx) (US.v idx) cell;
+  assert (is_dlist' pred (US.v hd) s' null FS.emptyset);
   if hd <> null_ptr then begin
-    lemma_dlist_insert_visited s' (US.v hd) (US.v idx) null FS.emptyset;
+    lemma_dlist_insert_visited pred s' (US.v hd) (US.v idx) null FS.emptyset;
     let fs1 = FS.singleton (US.v idx) in
     FS.all_finite_set_facts_lemma ();
     assert (fs1 `FS.equal` FS.insert (US.v idx) FS.emptyset);
-    assert (is_dlist' (US.v hd) s' null fs1);
+    assert (is_dlist' pred (US.v hd) s' null fs1);
     let cell = Seq.index s' (US.v hd) in
     let cell = {cell with prev = idx} in
     let cur = Seq.index s' (US.v hd) in
     let next = cur.next in
     let fs2 = FS.singleton (US.v hd) in
     assert (FS.insert (US.v hd) fs1 `FS.equal` FS.insert (US.v idx) fs2);
-    assert (is_dlist' (US.v next) s' (US.v hd) (FS.insert (US.v idx) fs2));
+    assert (is_dlist' pred (US.v next) s' (US.v hd) (FS.insert (US.v idx) fs2));
     // dedicated aux lemma
-    lemma_dlist_mem_uniq s' (US.v hd) null fs1;
+    lemma_dlist_mem_uniq pred s' (US.v hd) null fs1;
     assert (~ (mem' (US.v hd) (US.v next) s' (FS.insert (US.v idx) fs2)));
-    lemma_dlist_upd' s' (US.v next) (US.v hd) (US.v hd) (US.v hd) (FS.insert (US.v idx) fs2) cell;
+    lemma_dlist_upd' pred s' (US.v next) (US.v hd) (US.v hd) (US.v hd) (FS.insert (US.v idx) fs2) cell;
     let s1 = Seq.upd s' (US.v hd) cell in
-    assert (is_dlist' (US.v next) s1 (US.v hd) (FS.insert (US.v idx) fs2));
-    assert (is_dlist' (US.v hd) s1 (US.v idx) fs1
+    assert (is_dlist' pred (US.v next) s1 (US.v hd) (FS.insert (US.v idx) fs2));
+    assert (is_dlist' pred (US.v hd) s1 (US.v idx) fs1
     <==>
-    is_dlist' (US.v next) s1 (US.v hd) (FS.insert (US.v hd) fs1) /\
+    is_dlist' pred (US.v next) s1 (US.v hd) (FS.insert (US.v hd) fs1) /\
     (US.v (Seq.index s1 (US.v hd)).prev == US.v idx)
     );
     assert (US.v (Seq.index s1 (US.v hd)).prev == US.v idx);
-    let s2 = insert_spec s hd idx v in
+    let s2 = insert_spec pred s hd idx v in
     assert (s1 == s2);
     ()
   end else ()
@@ -528,6 +551,7 @@ let lemma_insert_spec (#a:Type)
 /// The resulting list is still a doubly linked list, and
 /// the element pointed to by [idx] was successfully removed
 val lemma_remove_spec' (#a:Type)
+  (pred: a -> prop)
   (hd:nat)
   (s:Seq.seq (cell a))
   (prev:nat)
@@ -535,26 +559,26 @@ val lemma_remove_spec' (#a:Type)
   (visited:FS.set nat{FS.cardinality visited <= Seq.length s})
   : Lemma (requires
             (forall i. FS.mem i visited ==> i < Seq.length s) /\
-            is_dlist' hd s prev visited /\
+            is_dlist' pred hd s prev visited /\
             mem' idx hd s visited /\
             null_or_valid prev s /\
             not (FS.mem idx visited))
           (ensures (
             let c = Seq.index s idx in
             let hd' = if hd = idx then US.v c.next else hd in
-            let s' = remove_spec hd s prev idx visited in
-            is_dlist' hd' s' prev visited /\
+            let s' = remove_spec pred hd s prev idx visited in
+            is_dlist' pred hd' s' prev visited /\
             ~ (mem' idx hd' s' visited)
           ))
           (decreases (Seq.length s - FS.cardinality visited))
 
-let rec lemma_remove_spec' #a hd s prev idx visited =
+let rec lemma_remove_spec' #a pred hd s prev idx visited =
   if hd = null then ()
   else begin
 
     let cur = Seq.index s hd in
     let next = US.v cur.next in
-    let s' = remove_spec hd s prev idx visited in
+    let s' = remove_spec pred hd s prev idx visited in
 
     // Base case, we are at the head of the list
     if hd = idx then begin
@@ -565,31 +589,31 @@ let rec lemma_remove_spec' #a hd s prev idx visited =
         let sint = Seq.upd s next nc in
 
         let fs = FS.insert hd visited in
-        assert (is_dlist' next s hd fs);
+        assert (is_dlist' pred next s hd fs);
         assert (next <> null);
 
         let next2 = US.v nc0.next in
-        assert (is_dlist' next2 s next (FS.insert next fs));
-        lemma_dlist_mem_uniq s next hd fs;
-        lemma_dlist_upd' s next2 next next next (FS.insert next fs) nc;
-        assert (is_dlist' next2 sint next (FS.insert next fs));
-        assert (is_dlist' next sint (US.v cur.prev) fs);
+        assert (is_dlist' pred next2 s next (FS.insert next fs));
+        lemma_dlist_mem_uniq pred s next hd fs;
+        lemma_dlist_upd' pred s next2 next next next (FS.insert next fs) nc;
+        assert (is_dlist' pred next2 sint next (FS.insert next fs));
+        assert (is_dlist' pred next sint (US.v cur.prev) fs);
 
-        lemma_mem_not_in_visited sint next (US.v cur.prev) fs hd;
+        lemma_mem_not_in_visited pred sint next (US.v cur.prev) fs hd;
         assert (~ (mem' hd next sint fs));
 
-        lemma_dlist_remove_visited sint next hd (US.v cur.prev) visited;
-        assert (is_dlist' next sint (US.v cur.prev) visited);
+        lemma_dlist_remove_visited pred sint next hd (US.v cur.prev) visited;
+        assert (is_dlist' pred next sint (US.v cur.prev) visited);
         assert (~ (mem' idx next sint visited));
 
         if US.v cur.prev = null then ()
         else begin
-          lemma_dlist_prev_not_mem sint next (US.v cur.prev) visited;
+          lemma_dlist_prev_not_mem pred sint next (US.v cur.prev) visited;
           assert (~ (mem' (US.v cur.prev) next sint visited));
           let pc0 = Seq.index s (US.v cur.prev) in
           let pc = {pc0 with next = cur.next} in
           assert (s' == Seq.upd sint (US.v cur.prev) pc);
-          lemma_dlist_upd' sint next (US.v cur.prev) (US.v cur.prev) idx visited pc
+          lemma_dlist_upd' pred sint next (US.v cur.prev) (US.v cur.prev) idx visited pc
         end
       end
     end
@@ -599,47 +623,48 @@ let rec lemma_remove_spec' #a hd s prev idx visited =
         let c = Seq.index s idx in
         let hd' = if next = idx then US.v c.next else next in
         let vis' = FS.insert hd visited in
-        lemma_remove_spec' next s hd idx vis';
-        assert (remove_spec hd s prev idx visited ==
-                remove_spec next s hd idx vis');
+        lemma_remove_spec' pred next s hd idx vis';
+        assert (remove_spec pred hd s prev idx visited ==
+                remove_spec pred next s hd idx vis');
 
-        assert (is_dlist' hd' s' hd vis');
+        assert (is_dlist' pred hd' s' hd vis');
         assert (~ (mem' idx hd' s' vis'));
 
         let cur' = Seq.index s' hd in
         if next = idx then begin
           assert (US.v c.prev == hd);
           assert (cur' == {cur with next = c.next});
-          assert (is_dlist' hd s' prev visited)
+          assert (is_dlist' pred hd s' prev visited)
         end else begin
-          lemma_mem_valid_or_null_next_prev' next s hd vis' idx;
-          lemma_mem_not_in_visited s next hd vis' hd;
+          lemma_mem_valid_or_null_next_prev' pred next s hd vis' idx;
+          lemma_mem_not_in_visited pred s next hd vis' hd;
           assert (~ (mem' hd next s vis'));
           assert (hd <> US.v c.next);
 
-          lemma_dlist_head_or_prev_not_visited next s hd vis' idx;
+          lemma_dlist_head_or_prev_not_visited pred next s hd vis' idx;
           assert (hd <> US.v c.prev);
 
           assert (cur' == cur);
-          assert (is_dlist' hd s' prev visited);
+          assert (is_dlist' pred hd s' prev visited);
           assert (~ (mem' idx hd s' visited))
         end
     end
   end
 
 val lemma_remove_spec (#a:Type)
+  (pred: a -> prop)
   (hd:nat)
   (s:Seq.seq (cell a))
   (idx:nat{idx < Seq.length s})
-  : Lemma (requires is_dlist hd s /\ mem idx hd s)
+  : Lemma (requires is_dlist pred hd s /\ mem idx hd s)
           (ensures (
             let c = Seq.index s idx in
             let hd' = if hd = idx then US.v c.next else hd in
-            let s' = remove_spec hd s null idx FS.emptyset in
-            is_dlist hd' s' /\ ~ (mem idx hd' s')
+            let s' = remove_spec pred hd s null idx FS.emptyset in
+            is_dlist pred hd' s' /\ ~ (mem idx hd' s')
           ))
 
-let lemma_remove_spec #a hd s idx = lemma_remove_spec' hd s null idx FS.emptyset
+let lemma_remove_spec #a pred hd s idx = lemma_remove_spec' pred hd s null idx FS.emptyset
 
 (** Steel functions and vprops *)
 
@@ -647,9 +672,8 @@ let lemma_remove_spec #a hd s idx = lemma_remove_spec' hd s null idx FS.emptyset
 /// We have access to an array, such that the array contains a doubly linked list
 /// when starting at offset [hd]
 [@@__steel_reduce__]
-let varraylist (#a:Type) (r:A.array (cell a)) (hd:nat) : vprop
-  = A.varray r `vrefine` (is_dlist hd)
-
+let varraylist (#a:Type) (pred: a -> prop) (r:A.array (cell a)) (hd:nat) : vprop
+  = A.varray r `vrefine` (is_dlist pred hd)
 
 /// AF: The regular noop does not seem to pick the equality of selectors, not sure why
 val noop (#opened:inames) (#p:vprop) (_:unit)
@@ -659,61 +683,63 @@ let noop () = noop ()
 /// Reads at index [idx] in the array.
 /// TODO: The hd pointer should be ghost
 val read_in_place (#a:Type)
+  (#pred: a -> prop)
   (r:A.array (cell a))
   (hd:nat)
   (idx:US.t{US.v idx < A.length r})
   : Steel a
-          (varraylist r hd)
-          (fun _ -> varraylist r hd)
+          (varraylist pred r hd)
+          (fun _ -> varraylist pred r hd)
           (requires fun _ -> True)
-          (ensures fun h0 _ h1 -> h0 (varraylist r hd) == h1 (varraylist r hd))
+          (ensures fun h0 _ h1 -> h0 (varraylist pred r hd) == h1 (varraylist pred r hd))
 
-let read_in_place #a r hd idx =
-  (**) elim_vrefine (A.varray r) (is_dlist hd);
+let read_in_place #a #pred r hd idx =
+  (**) elim_vrefine (A.varray r) (is_dlist pred hd);
   let res = A.index r idx in
-  (**) intro_vrefine (A.varray r) (is_dlist hd);
+  (**) intro_vrefine (A.varray r) (is_dlist pred hd);
   (**) return res.data
 
 
 /// Updates the `data` field of the cell at index [idx] in the array [r] with [v]
 /// TODO: The hd pointer should be ghost
 val write_in_place (#a:Type)
+  (#pred: a -> prop)
   (r:A.array (cell a))
   (hd:nat)
   (idx:US.t{US.v idx < A.length r})
   (v:a)
    : Steel unit
-          (varraylist r hd)
-          (fun _ -> varraylist r hd)
-          (requires fun _ -> True)
+          (varraylist pred r hd)
+          (fun _ -> varraylist pred r hd)
+          (requires fun _ -> pred v)
           (ensures fun h0 _ h1 -> True) // TODO
 
-let write_in_place #a r hd idx v =
-  (**) elim_vrefine (A.varray r) (is_dlist hd);
+let write_in_place #a #pred r hd idx v =
+  (**) elim_vrefine (A.varray r) (is_dlist pred hd);
   let c = A.index r idx in
   (**) let gs = gget (A.varray r) in
   A.upd r idx (write_data c v);
-  (**) lemma_write_data_frame hd gs (US.v idx) v;
-  (**) intro_vrefine (A.varray r) (is_dlist hd)
-
+  (**) lemma_write_data_frame pred hd gs (US.v idx) v;
+  (**) intro_vrefine (A.varray r) (is_dlist pred hd)
 
 /// Removes the element at offset [idx] from the dlist pointed to by [hd]
 val remove (#a:Type)
+  (#pred: a -> prop)
   (r:A.array (cell a))
   (hd:nat)
   (idx:US.t{US.v idx < A.length r})
    : Steel nat
-          (varraylist r hd)
-          (fun hd' -> varraylist r hd')
-          (requires fun h -> mem (US.v idx) hd (h (varraylist r hd)))
+          (varraylist pred r hd)
+          (fun hd' -> varraylist pred r hd')
+          (requires fun h -> mem (US.v idx) hd (h (varraylist pred r hd)))
           (ensures fun h0 hd' h1 ->
-            ~ (mem (US.v idx) hd' (h1 (varraylist r hd')))) // TODO
+            ~ (mem (US.v idx) hd' (h1 (varraylist pred r hd')))) // TODO
 
-let remove #a r hd idx =
-  (**) elim_vrefine (A.varray r) (is_dlist hd);
+let remove #a #pred r hd idx =
+  (**) elim_vrefine (A.varray r) (is_dlist pred hd);
   (**) let gs0 = gget (A.varray r) in
   let cell = A.index r idx in
-  (**) lemma_mem_valid_or_null_next_prev hd gs0 (US.v idx);
+  (**) lemma_mem_valid_or_null_next_prev pred hd gs0 (US.v idx);
 
   if cell.next <> null_ptr then
     // Next is not null, we need to update it
@@ -731,28 +757,29 @@ let remove #a r hd idx =
 
   (**) let gs1 = gget (A.varray r) in
   let hd' = if hd = US.v idx then US.v cell.next else hd in
-  (**) lemma_remove_spec hd gs0 (US.v idx);
+  (**) lemma_remove_spec pred hd gs0 (US.v idx);
 
-  (**) intro_vrefine (A.varray r) (is_dlist hd');
+  (**) intro_vrefine (A.varray r) (is_dlist pred hd');
   return hd'
 
 
 /// Assuming the element at offset [idx] does not belong to the dlist,
 /// insert it at the head
 val insert (#a:Type)
+  (#pred: a -> prop)
   (r:A.array (cell a))
   (hd:US.t{hd == null_ptr \/ US.v hd < A.length r})
   (idx:US.t{idx <> null_ptr /\ US.v idx < A.length r})
   (v: a)
    : Steel unit
-          (varraylist r (US.v hd))
-          (fun _ -> varraylist r (US.v idx))
-          (requires fun h -> ~ (mem (US.v idx) (US.v hd) (h (varraylist r (US.v hd)))))
+          (varraylist pred r (US.v hd))
+          (fun _ -> varraylist pred r (US.v idx))
+          (requires fun h -> pred v /\ (~ (mem (US.v idx) (US.v hd) (h (varraylist pred r (US.v hd))))))
           (ensures fun h0 hd' h1 ->
-            mem (US.v idx) (US.v idx) (h1 (varraylist r (US.v idx)))) // TODO
+            mem (US.v idx) (US.v idx) (h1 (varraylist pred r (US.v idx)))) // TODO
 
-let insert #a r hd idx v =
-  (**) elim_vrefine (A.varray r) (is_dlist (US.v hd));
+let insert #a #pred r hd idx v =
+  (**) elim_vrefine (A.varray r) (is_dlist pred (US.v hd));
   (**) let gs0 = gget (A.varray r) in
 
   let cell = {data = v; prev = null_ptr; next = hd} in
@@ -763,5 +790,5 @@ let insert #a r hd idx v =
     A.upd r hd cell
   else noop ();
 
-  (**) lemma_insert_spec gs0 hd idx v;
-  (**) intro_vrefine (A.varray r) (is_dlist (US.v idx))
+  (**) lemma_insert_spec pred gs0 hd idx v;
+  (**) intro_vrefine (A.varray r) (is_dlist pred (US.v idx))
